src/ISAR/HFSetSemantics.lean
@@ -1,4 +1,4 @@
-import HFSetEncoding
+import ISAR.HFSetEncoding
 
 namespace ISAR
 
